verity/proof/Tamago/Proof.lean
@@ -4,5 +4,4 @@ import Tamago.Proof.Tokens.ERC20Proof
 import Tamago.Proof.Tokens.ERC721Proof
 import Tamago.Proof.Tokens.ERC4626Proof
 import Tamago.Proof.Tokens.WETHProof
-import Tamago.Utils.ClzIntrinsic
 import Tamago.Proof.Utils.FixedPointMathLibProof
